frontend/coq_pp.ml
@@ -110,23 +110,25 @@ let pp_un_op : Coq_ast.un_op pp = fun ff op ->
 let pp_bin_op : Coq_ast.bin_op pp = fun ff op ->
   pp_str ff @@
   match op with
-  | AddOp       -> "+"
-  | SubOp       -> "-"
-  | MulOp       -> "×"
-  | DivOp       -> "/"
-  | ModOp       -> "%"
-  | AndOp       -> "&"
-  | OrOp        -> "|"
-  | XorOp       -> "^"
-  | ShlOp       -> "<<"
-  | ShrOp       -> ">>"
-  | EqOp        -> "="
-  | NeOp        -> "!="
-  | LtOp        -> "<"
-  | GtOp        -> ">"
-  | LeOp        -> "≤"
-  | GeOp        -> "≥"
-  | CommaOp     -> ","
+  | AddOp     -> "+"
+  | SubOp     -> "-"
+  | MulOp     -> "×"
+  | DivOp     -> "/"
+  | ModOp     -> "%"
+  | AndOp     -> "&"
+  | OrOp      -> "|"
+  | XorOp     -> "^"
+  | ShlOp     -> "<<"
+  | ShrOp     -> ">>"
+  | EqOp      -> "="
+  | NeOp      -> "!="
+  | LtOp      -> "<"
+  | GtOp      -> ">"
+  | LeOp      -> "≤"
+  | GeOp      -> "≥"
+  | CommaOp   -> ","
+  | LazyAndOp -> "&&"
+  | LazyOrOp  -> "||"
 
 let rec pp_expr : Coq_ast.expr pp = fun ff e ->
   let pp fmt = Format.fprintf ff fmt in
@@ -278,11 +280,11 @@ let rec pp_stmt : Coq_ast.stmt pp = fun ff stmt ->
         pp_expr e1 pp_op_type ot order pp_expr e2 pp_stmt stmt
   | SkipS(stmt)                   ->
       pp_stmt ff stmt
-  | If(e,stmt1,stmt2)             ->
-      pp "if: @[<hov 0>%a@]@;then@;@[<v 2>%a@]@;else@;@[<v 2>%a@]"
-        pp_expr e pp_stmt stmt1 pp_stmt stmt2
-  | Assert(e, stmt)               ->
-      pp "assert: (%a) ;@;%a" pp_expr e pp_stmt stmt
+  | If(ot,e,stmt1,stmt2)          ->
+      pp "if{%a}: @[<hov 0>%a@]@;then@;@[<v 2>%a@]@;else@;@[<v 2>%a@]"
+        pp_op_type ot pp_expr e pp_stmt stmt1 pp_stmt stmt2
+  | Assert(ot,e,stmt)             ->
+      pp "assert{%a}: (%a) ;@;%a" pp_op_type ot pp_expr e pp_stmt stmt
   | ExprS(annot, e, stmt)         ->
       Option.iter (Option.iter (pp "annot: (%s) ;@;")) annot;
       pp "expr: (%a) ;@;%a" pp_expr e pp_stmt stmt
